ulib/FStar.SL.fst
@@ -22,20 +22,13 @@ type disjoint (h1:heap) (h2:heap) =
   ((forall (a:Type0) (r:ref a). (h1 `contains` r) <==> (r `unused_in` h2)) 
     /\ (forall (a:Type0) (r:ref a). (h2 `contains` r) <==> (r `unused_in` h1)))
 
-type heap_pair = heap * heap
+type star (p:predicate) (q:predicate) (h:heap) =
+  (exists h1 h2. (p h1) /\ (q h2) /\ (disjoint h1 h2) /\ (same h (join h1 h2)))
 
-let join (h:heap_pair) : Type0 = 
-  match h with
-  | (h1, h2) -> (disjoint h1 h2)
-  
-let star (p:predicate) (q:predicate) (h:heap_pair) : Type0 =
-  match h with
-  | (h1, h2) -> ((p h1) /\ (q h2) /\ (join h))
-
-val lemma_frame_rule: h0:heap -> h1:heap -> h2:heap -> p:predicate -> q:predicate -> r:predicate 
-  -> Lemma (requires ((p h0 ==> q h1) /\ (disjoint h1 h2)))
-           (ensures ((star p r (h0, h2)) ==> (star q r (h1, h2))))
-let lemma_frame_rule h0 h1 h2 p q r = ()
+val lemma_frame_rule: p:predicate -> q:predicate -> r:predicate -> h1:heap -> h2:heap
+  -> Lemma (requires (p h1 ==> q h1) /\ (disjoint h1 h2) /\ (p h1) /\  (r h2))
+           (ensures (star p r (join h1 h2)) ==> (star q r (join h1 h2)))
+let lemma_frame_rule p q r h1 h2 = ()
 
 val lemma_alloc_rule: #a:Type0 -> h:heap -> v:a
   -> Lemma (requires (empty_heap h))
@@ -45,5 +38,5 @@ let lemma_alloc_rule #a h v = ()
 
 val lemma_sequencing_rule: p:predicate -> h:heap
  -> Lemma (requires (p h))
-          (ensures (star p (empty_heap) (h, emp)))
+          (ensures (star p (empty_heap) (join h emp)))
 let lemma_sequencing_rule p h = ()
